{
 "cells": [
  {
   "cell_type": "markdown",
   "metadata": {},
   "source": [
    "# MATH535 HW9\n",
    "#### Lingyu Zhou\n",
    "##### 2023.4.17\n",
    "<span style=\"color:red\"><small> **Any kind of reuse or transmission is prohibited!** </small><span>\n",
    "<hr>"
   ]
  },
  {
   "cell_type": "markdown",
   "metadata": {},
   "source": [
    "## Problem 1\n",
    "### i.\n",
    "\n",
    "According to the definition, we have for any matrix $A\\in \\mathbb{R}^{m \\times n}$:\n",
    "\n",
    "$$\n",
    "\\begin{align}\n",
    "tr(A^TA)&=\\sum_{i=1}^m (A^TA)_{ii}\\\\\n",
    "&=\\sum_{i=1}^m \\sum_{j=1}^n A^T_{ij}A_{ji}\\\\\n",
    "&=\\sum_{i=1}^m \\sum_{j=1}^n A_{ji}A_{ji}\\\\\n",
    "&=\\sum_{i=1}^m \\sum_{j=1}^n A_{ji}^2,\\\\\n",
    "\\end{align}\n",
    "$$\n",
    "\n",
    "which is the definition of F-norm squared, namely the sum of all entries squared.\n",
    "\n",
    "Therefore, we have:\n",
    "$$\n",
    "\\begin{align}\n",
    "||Y-XB||^2_F-\\lambda ||B||^2_F&=tr((Y-XB)^T(Y-XB))-\\lambda(tr(B^TB))\\\\\n",
    "&=tr((Y^T-B^TX^T)(Y-XB))-\\lambda(tr(B^TB))\\\\\n",
    "&=tr((Y^TY-Y^TXB-B^TX^TY+B^TX^TXB))-\\lambda(tr(B^TB))\\\\\n",
    "&=tr(Y^TY)-tr(Y^TXB)-tr(B^TX^TY)+tr(B^TX^TXB)-\\lambda(tr(B^TB))\\\\\n",
    "&=tr(Y^TY)-tr(Y^TXB)-tr((Y^TXB)^T)+tr(B^TX^TXB)-\\lambda(tr(B^TB))\\\\\n",
    "&=tr(Y^TY)-2tr(Y^TXB)+tr(B^TX^TXB)-\\lambda(tr(B^TB)),\\\\\n",
    "\\end{align}\n",
    "$$\n",
    "as desired."
   ]
  },
  {
   "cell_type": "markdown",
   "metadata": {},
   "source": [
    "### ii.\n",
    "$$\n",
    "\\begin{align}\n",
    "\\frac{\\partial}{\\partial B} (||Y-XB||^2_F+\\lambda ||B||^2_F)&=\\frac{\\partial}{\\partial B}[tr(Y^TY)-2tr(Y^TXB)+tr(B^TX^TXB)+\\lambda tr(B^TB)]\\\\\n",
    "&=\\frac{\\partial}{\\partial B}tr(Y^TY)-\\frac{\\partial}{\\partial B}2tr(Y^TXB)+\\frac{\\partial}{\\partial B}tr(B^TX^TXB)+\\frac{\\partial}{\\partial B}\\lambda tr(B^TB)\\\\\n",
    "&=0-2\\frac{\\partial}{\\partial B}tr[(Y^T)XB]+\\frac{\\partial}{\\partial B}tr[B^T(X^TX)B]+\\lambda \\frac{\\partial}{\\partial B} tr(B^TIB)\\\\\n",
    "&=-2(X^TYI)+(X^TXB+X^TXB)+\\lambda(IB+IB)\\\\\n",
    "&=-2(X^TY)+2(X^TXB)+\\lambda(2B)\\\\\n",
    "&=2(X^TX+\\lambda I)B-2X^TY,\n",
    "\\end{align}\n",
    "$$\n",
    "as desired. \n",
    "\n",
    "And then we can easily get:\n",
    "$$\n",
    "\\begin{align}\n",
    "\\frac{\\partial^2}{\\partial B^2} (||Y_XB||^2_F+\\lambda ||B||^2_F)&=\\frac{\\partial}{\\partial B}[2(X^TX+\\lambda I)B-2X^TY]\\\\\n",
    "&=2\\frac{\\partial}{\\partial B}[(X^TX+\\lambda I)BI-2X^TY]\\\\\n",
    "&=2(X^TX+\\lambda I)^T-0\\\\\n",
    "&=2[(X^TX)^T+(\\lambda I)^T]\\\\\n",
    "&=2(X^TX+\\lambda I),\n",
    "\\end{align}\n",
    "$$\n",
    "as desired."
   ]
  },
  {
   "cell_type": "markdown",
   "metadata": {},
   "source": [
    "### iii.\n",
    "According to $\\textbf{Proposition 7}$ from the \\textcolor{magenta}{Ref}, to show $||Y-XB||^2_F$ is convex, it suffices to show $\\frac{\\partial^2}{\\partial B^2} ||Y-XB||^2_F \\succcurlyeq 0$:\n",
    "\n",
    "$$\n",
    "\\begin{align}\n",
    "\\frac{\\partial^2}{\\partial B^2} ||Y-XB||^2_F &=\\frac{\\partial}{\\partial B} -2X^TY+2X^TXB\\\\\n",
    "&=\\frac{\\partial}{\\partial B} 2(X^TX)BI\\\\\n",
    "&=2(X^TX)^TI^T\\\\\n",
    "&=2(X^TX)\n",
    "\\end{align}\n",
    "$$\n",
    "$\\forall w \\in \\mathbb{R}^r \\neq \\vec{0}$:\n",
    "$$\n",
    "\\begin{align}\n",
    "w^T[2(X^TX)]w&=2w^TX^TXw\\\\\n",
    "&=2(Xw)^TXw\\\\\n",
    "&=2||Xw||^2\\\\\n",
    "&\\succcurlyeq 0\n",
    "\\end{align}\n",
    "$$\n",
    "\n",
    "Hence by $\\textbf{Corollary }6$, every critical point $x*$, when $\\nabla f(x*)=0$, is a global minimizer, hence a local minimizer, where $f:B\\mapsto ||Y-XB||^2_F$."
   ]
  },
  {
   "cell_type": "markdown",
   "metadata": {},
   "source": [
    "#### iv.\n",
    "\n",
    "By $\\textbf{Corollary }6$, if $\\nabla f(B*)=0$, and we've already shown that $f$ is convex, then $B*$ is a global minimizer:\n",
    "$$\n",
    "\\begin{align}\n",
    "\\nabla f= \\frac{\\partial}{\\partial B} ||Y-BX||^2_F&=0\\\\\n",
    "\\Rightarrow -2X^TY+2(X^TXB)&=0\\\\\n",
    "X^TXB&=X^TY\\\\\n",
    "B&=(X^TX)^{-1}X^TY\n",
    "\\end{align}\n",
    "$$"
   ]
  },
  {
   "cell_type": "markdown",
   "metadata": {},
   "source": [
    "### v.\n",
    "To show $X^TX+\\lambda I$ is invertible, it suffices to show that $X^TX+\\lambda I$ is positive definite. $\\forall w \\in \\mathbb{R}^r \\neq \\vec{0}$:\n",
    "$$\n",
    "\\begin{align}\n",
    "w^T(X^TX+\\lambda I)w&=(w^TX^TX+w^T\\lambda I)w\\\\\n",
    "&=w^TX^TXw+w^T\\lambda Iw\\\\\n",
    "&=(Xw)^TXw+\\lambda w^Tw\\\\\n",
    "&=||Xw||^2+\\lambda||w||^2\\\\\n",
    "&\\succ 0,\n",
    "\\end{align}\n",
    "$$\n",
    "\n",
    "where (39) comes from $w \\neq \\vec{0}$ and $\\lambda >0$\\\\\n",
    "\\\\Therefore, $X^TX+\\lambda I$ always has an inverse.\n",
    "Similarly as in \\textbf{iv.}, we need to find the $ \\tilde{B*}$ as a global minimizer s.t. $\\nabla \\tilde{f}(\\tilde{B*})=0$:\n",
    "$$\n",
    "\\begin{align}\n",
    "\\nabla \\tilde{f}=\\frac{\\partial}{\\partial B} ||Y-BX||^2_F+||B||^2_F&=0\\\\\n",
    "\\Rightarrow 2(X^TX+\\lambda I)B-2X^TY&=0\\\\\n",
    "(X^TX+\\lambda I)B&=X^TY\\\\\n",
    "B&=(X^TX+\\lambda I)^{-1}X^TY,\n",
    "\\end{align}\n",
    "$$\n",
    "$Q.E.D$"
   ]
  },
  {
   "cell_type": "markdown",
   "metadata": {},
   "source": [
    "## Problem 2\n",
    "### i.\n",
    "Suppose $B\\in \\mathbb{R}^{n \\times l}$, $X\\in \\mathbb{R}^{l \\times m}$, $C\\in \\mathbb{R}^{m\\times n}, \\forall x_{pq} \\in X:$\n",
    "\n",
    "$$\n",
    "\\begin{align}\n",
    "\\frac{\\partial}{\\partial x_{pq}} \n",
    "tr(BXC)&=\\frac{\\partial}{\\partial x_{pq}} \\sum_{i=1}^n (BXC)_{ii}\\\\\n",
    "&=\\frac{\\partial}{\\partial x_{pq}} \\sum_{i=1}^n \\sum_{j=1}^l  B_{ij}(XC)_{ji}\\\\\n",
    "&=\\frac{\\partial}{\\partial x_{pq}} \\sum_{i=1}^n \\sum_{j=1}^l   \\sum_{k=1}^m  B_{ij}X_{jk} C_{ki}\\\\\n",
    "&=\\frac{\\partial}{\\partial x_{pq}} \\sum_{i=1}^n \\sum_{j=1}^l   \\sum_{k=1}^m  B_{ij}x_{jk} C_{ki}\\\\\n",
    "&= 0+ \\frac{\\partial}{\\partial x_{pq}}\\sum_{i=1}^n B_{ip}C_{qi}\\\\\n",
    "&=\\sum_{i=1}^n  B^T_{pi}C^T_{iq}\\\\\n",
    "&=(B^TC^T)_{pq}\n",
    "\\end{align}\n",
    "$$\n",
    "\n",
    "Therefore:\n",
    "$$\n",
    "\\frac{\\partial}{\\partial X} tr(BXC)=B^TC^T,\n",
    "$$\n",
    "\n",
    "as desired.\n",
    "\n",
    "Suppose $X$ is of the same dimension, so that $X^T \\in \\mathbb{R}^{m \\times 1} $ now let $\\tilde{B}\\in \\mathbb{R}^{n \\times m}$, $\\tilde{C} \\in \\mathbb{R}^{l \\times n}$ so that $BX^TC \\in \\mathbb{R}^{n \\times n}$. Therefore:\n",
    "\n",
    "$$\n",
    "\\begin{align}\n",
    "tr(\\tilde{B}X^T\\tilde{C})&=tr[(\\tilde{B}X^T\\tilde{C})^T]\\\\\n",
    "&=tr(\\tilde{C}^TX\\tilde{B}^T),\n",
    "\\end{align}\n",
    "$$\n",
    "\n",
    "where we can find out $\\tilde{C}^T \\in \\mathbb{R}^{n \\times l}$, $\\tilde{B}^T \\in \\mathbb{R}^{m \\times n}$, which satisfies the condition in of matrices in $(i)$. Using the conclusion from $(i)$, we can then get:\n",
    "\n",
    "$$\n",
    "\\frac{\\partial}{\\partial X} tr(BX^TC)=CB,\n",
    "$$\n",
    "as desired."
   ]
  },
  {
   "cell_type": "markdown",
   "metadata": {},
   "source": [
    "# ii.\n",
    "Suppose $X\\in \\mathbb{R}^{m \\times n}$, $X^T\\in \\mathbb{R}^{n \\times m}$, meaning  $B\\in \\mathbb{R}^{m\\times m}, \\forall x_{pq} \\in X\\in \\mathbb{R}^{m \\times n}:$\n",
    "\n",
    "$$\n",
    "\\begin{align}\n",
    "\\frac{\\partial}{\\partial x_{pq}} tr(X^TBX)&=\\frac{\\partial}{\\partial x_{pq}} \\sum_{i=1}^n (X^TBX)_{ii}\\\\\n",
    "&=\\frac{\\partial}{\\partial x_{pq}} \\sum_{i=1}^n \\sum_{j=1}^m (X^TB)_{ij}X_{ji}\\\\\n",
    "&=\\frac{\\partial}{\\partial x_{pq}}  \\sum_{i=1}^n \\sum_{j=1}^m \\sum_{k=1}^m X^T_{ik} B_{kj} X_{ji}\\\\\n",
    "&=\\frac{\\partial}{\\partial x_{pq}}  \\sum_{i=1}^n \\sum_{j=1}^m \\sum_{k=1}^m B_{kj}(x_{ki} x_{ji})\\\\\n",
    "&=\\underbrace{\\frac{\\partial}{\\partial x_{pq}} B_{pp} x_{pq}^2}_\\text{$k=j=p,i=q$}+\\underbrace{\\frac{\\partial}{\\partial x_{pq}}  \\sum_{j=1}^m B_{pj} x_{pq} x_{jq}}_\\text{$p=k\\neq j,i=q$}+\\ \n",
    "\\underbrace{\\frac{\\partial}{\\partial x_{pq}}  \\sum_{k=1}^m B_{kp} x_{kq} x_{pq}}_\\text{$p=j\\neq k,i=q$}\\\\\n",
    "&= 2B_{pp}x_{pq}+\\sum_{j=1}^m B_{pj} x_{jq} +\\sum_{k=1}^m B_{kp} x_{kq}\\\\\n",
    "&= \\sum_{j=1}^m B_{pj} x_{jq} +\\sum_{k=1}^m B_{kp} x_{kq}\\\\\n",
    "&=\\sum_{j=1}^m B_{pj} X_{jq} +\\sum_{k=1}^m B^T_{pk} X_{kq}\\\\\n",
    "&=BX+B^TX,\n",
    "\\end{align}\n",
    "$$\n",
    "\n",
    "as desired.\n",
    "$\\textbf{Note that in (60)}$ term $2B_{pp}x_{pq}$ goes away because we distribute the it into 2 $B_{pp}x_{pq}|_{p=j}$ and $B_{pp}x_{pq}|_{p=k}$ that combine correspondingly with the latter 2 terms in $(59)$ to make them in full matrix multiplication form.\n",
    "\n",
    "Let $C\\in \\mathbb{R}^{l \\times l}$, the new $X\\in \\mathbb{R}^{l \\times m}$ so that $CX \\in \\mathbb{R}^{l\\times m}$, and $X^TC\\in \\mathbb{R}^{m \\times l}$. So the new $B \\in \\mathbb{R}^{m \\times n}$. Let $\\tilde{X}=XB$ and $I \\in \\mathbb{R}^{l \\times l}$ to be the identity matrix, we have:\n",
    "\n",
    "$$\n",
    "\\begin{align}\n",
    "\\frac{\\partial}{\\partial X}tr(B^TX^TCXB)&=\\frac{\\partial}{\\partial X}tr[(XB)^TC(XB)]\\\\\n",
    "&=\\frac{\\partial}{\\partial X}tr(\\tilde{X}^TC\\tilde{X})\\\\\n",
    "&=(C\\tilde{X}+C^T\\tilde{X})\\frac{\\partial }{\\partial X} tr(\\tilde{X})\\\\\n",
    "&=(C\\tilde{X}+C^T\\tilde{X})\\frac{\\partial }{\\partial X} tr(XB)\\\\\n",
    "&=(C\\tilde{X}+C^T\\tilde{X})\\frac{\\partial }{\\partial X}tr({IXB})\\\\\n",
    "&=(C\\tilde{X}+C^T\\tilde{X})(I^TB^T)\\\\\n",
    "&=(CXB+C^TXB)B^T\\\\\n",
    "&=CXBB^T+C^TXBB^T,\n",
    "\\end{align}\n",
    "$$\n",
    "\n",
    "as desired.\n",
    "Note that we use chain rule from Ref: [The Matrix Cookbook](https://www.math.uwaterloo.ca/~hwolkowi/matrixcookbook.pdf) **Petersen & Pedersen, 2012, p. 15** for $(30)$, and the conclusion from the previous part in (ii) for $(33)$"
   ]
  },
  {
   "cell_type": "markdown",
   "metadata": {},
   "source": [
    "## Problem 3\n",
    "\n",
    "Write\n",
    "\n",
    "$$\n",
    "X=\n",
    "\\begin{bmatrix}\n",
    "X_1\\\\\n",
    "\\vdots\\\\\n",
    "X_N\\\\\n",
    "\\end{bmatrix}\n",
    "$$\n",
    "\n",
    "From definition:\n",
    "$$\n",
    "\\begin{align}\n",
    "L(y_1,\\cdots, y_N;w,\\sigma)&=\\prod_{i=1}^N F(\\hat{Y}_i=y_i)|_{\\hat{Y}_i(x_i;w,\\sigma)\\sim N(\\phi(x)^Tw,\\sigma ^2)}\\\\\n",
    "&=\\prod_{i=1}^N F(\\hat{Y}_i=y_i)|_{\\hat{Y}_i(x_i;w,\\sigma)\\sim N(\\sum_{i=0}^M x^iw_i,\\sigma ^2)}\\\\\n",
    "&=\\prod_{i=1}^N \\frac{1}{\\sigma \\sqrt{2 \\pi}} \\exp{\\left[-\\frac{(y_i-\\sum_{j=0}^M x^jw_j)^2}{2\\sigma ^2}\\right]}\\\\\n",
    "&=\\left(\\frac{1}{\\sigma \\sqrt{2 \\pi}}\\right) ^N \\prod_{i=1}^N \\exp{\\left[-\\frac{(y_i-\\sum_{j=0}^M x^jw_j)^2}{2\\sigma ^2}\\right]}\\\\\n",
    "&=(\\sigma^2 2\\pi)^{-\\frac{N}{2}} \\exp{\\left\\{ -\\frac{1}{2\\sigma^2} \\left[ \\sum_{i=1}^N (y_i- \\sum_{j=0}^M x^jw_j)^2\\right]\\right\\}}\\\\\n",
    "&=(\\sigma^2 2\\pi)^{-\\frac{N}{2}} \\exp{\\left[ -\\frac{1}{2\\sigma^2}  \\sum_{i=1}^N (y_i- X_i^Tw)^2\\right]}\\\\\n",
    "&=(\\sigma^2 2\\pi)^{-\\frac{N}{2}} \\exp{\\left\\{ -\\frac{1}{2\\sigma^2}  \\sum_{i=1}^N [Y_i-(Xw)_i]^2\\right\\}}\\\\\n",
    "&=(\\sigma^2 2\\pi)^{-\\frac{N}{2}} \\exp{\\left[ -\\frac{1}{2\\sigma^2}  ||Y-Xw||^2_F\\right]},\n",
    "\\end{align}\n",
    "$$\n",
    "as desired."
   ]
  }
 ],
 "metadata": {
  "language_info": {
   "name": "python"
  },
  "orig_nbformat": 4
 },
 "nbformat": 4,
 "nbformat_minor": 2
}
